Foundation/Modal/Kripke/Completeness.lean
@@ -1,70 +1,70 @@
-import Foundation.Modal.Hilbert.ConsistentTheory
+import Foundation.Modal.MaximalConsistentSet
 import Foundation.Modal.Kripke.Basic
 
 namespace LO.Modal
 
 open System
 open Formula
-open MaximalConsistentTheory
-open Hilbert.Deduction
 open Kripke
+open MaximalConsistentSet
 
-variable {H : Hilbert ℕ} [H.IsNormal] [H.Consistent]
-
-namespace Hilbert
+variable {S} [System (Formula ℕ) S]
+variable {𝓢 : S} [System.Consistent 𝓢] [System.K 𝓢]
 
 namespace Kripke
 
-abbrev canonicalFrame (H : Hilbert ℕ) [H.IsNormal] [H.Consistent] : Kripke.Frame where
-  World := MCT H
-  Rel Ω₁ Ω₂ := □''⁻¹Ω₁.theory ⊆ Ω₂.theory
+abbrev canonicalFrame (𝓢 : S) [System.Consistent 𝓢] [System.K 𝓢] : Kripke.Frame where
+  World := MaximalConsistentSet 𝓢
+  Rel X Y := □''⁻¹X.1 ⊆ Y.1
 
 namespace canonicalFrame
 
-variable {Ω₁ Ω₂ : (canonicalFrame H).World}
+variable {Ω₁ Ω₂ : (canonicalFrame 𝓢).World}
 
-@[simp] lemma rel_def_box: Ω₁ ≺ Ω₂ ↔ ∀ {φ}, □φ ∈ Ω₁.theory → φ ∈ Ω₂.theory := by simp [Frame.Rel']; aesop;
+@[simp] lemma rel_def_box: Ω₁ ≺ Ω₂ ↔ ∀ {φ}, □φ ∈ Ω₁ → φ ∈ Ω₂ := by simp [Frame.Rel']; aesop;
 
-lemma multirel_def_multibox : Ω₁ ≺^[n] Ω₂ ↔ ∀ {φ}, □^[n]φ ∈ Ω₁.theory → φ ∈ Ω₂.theory := by
+lemma multirel_def_multibox : Ω₁ ≺^[n] Ω₂ ↔ ∀ {φ}, □^[n]φ ∈ Ω₁.1 → φ ∈ Ω₂.1 := by
   induction n generalizing Ω₁ Ω₂ with
   | zero =>
     simp_all only [Rel.iterate.iff_zero, Function.iterate_zero, id_eq];
     constructor;
-    . intro h; subst h; tauto;
-    . intro h; apply intro_equality; simpa;
+    . intro h; tauto_set;
+    . intro h;
+      apply intro_equality;
+      tauto_set;
   | succ n ih =>
     constructor;
     . intro h φ hp;
       obtain ⟨⟨Ω₃, _⟩, R₁₃, R₃₂⟩ := h;
       apply ih.mp R₃₂ $ rel_def_box.mp R₁₃ (by simpa using hp);
     . intro h;
-      obtain ⟨Ω, hΩ⟩ := lindenbaum (H := H) (T := (□''⁻¹Ω₁.theory ∪ ◇''^[n]Ω₂.theory)) $ by
-        apply Theory.intro_union_consistent;
+      obtain ⟨Ω, hΩ⟩ := lindenbaum (𝓢 := 𝓢) (T := (□''⁻¹Ω₁.1 ∪ ◇''^[n]Ω₂.1)) $ by
+        apply FormulaSet.intro_union_consistent;
         rintro Γ Δ ⟨hΓ, hΔ⟩ hC;
 
-        replace hΓ : ∀ φ ∈ Γ, □φ ∈ Ω₁.theory := by simpa using hΓ;
-        have dΓconj : Ω₁.theory *⊢[H]! □⋀Γ := membership_iff.mp $ iff_mem_box_conj.mpr hΓ;
+        replace hΓ : ∀ φ ∈ Γ, □φ ∈ Ω₁ := by simpa using hΓ;
+        have dΓconj : Ω₁.1 *⊢[𝓢]! □⋀Γ := membership_iff.mp $ iff_mem_box_conj.mpr hΓ;
 
-        have hΔ₂ : ∀ φ ∈ ◇'⁻¹^[n]Δ, φ ∈ Ω₂.theory := by
+        have hΔ₂ : ∀ φ ∈ ◇'⁻¹^[n]Δ, φ ∈ Ω₂ := by
           intro φ hp;
           exact Set.iff_mem_multidia.mp $ hΔ (◇^[n]φ) (by simpa using hp);
 
-        have hΔconj : ⋀◇'⁻¹^[n]Δ ∈ Ω₂.theory := iff_mem_conj.mpr hΔ₂;
+        have hΔconj : ⋀◇'⁻¹^[n]Δ ∈ Ω₂ := iff_mem_conj.mpr hΔ₂;
 
-        have : ⋀◇'⁻¹^[n]Δ ∉ Ω₂.theory := by {
-          have d₁ : H ⊢! ⋀Γ ➝ ⋀Δ ➝ ⊥ := and_imply_iff_imply_imply'!.mp hC;
-          have : H ⊢! ⋀(◇'^[n]◇'⁻¹^[n]Δ) ➝ ⋀Δ := by
+        have : ⋀◇'⁻¹^[n]Δ ∉ Ω₂ := by {
+          have d₁ : 𝓢 ⊢! ⋀Γ ➝ ⋀Δ ➝ ⊥ := and_imply_iff_imply_imply'!.mp hC;
+          have : 𝓢 ⊢! ⋀(◇'^[n]◇'⁻¹^[n]Δ) ➝ ⋀Δ := by
             apply conjconj_subset!;
             intro ψ hq;
             obtain ⟨χ, _, _⟩ := hΔ ψ hq;
             subst_vars;
             simpa;
-          have : H ⊢! ◇^[n]⋀◇'⁻¹^[n]Δ ➝ ⋀Δ := imp_trans''! iff_conjmultidia_multidiaconj! $ this;
-          have : H ⊢! ∼(□^[n](∼⋀◇'⁻¹^[n]Δ)) ➝ ⋀Δ := imp_trans''! (and₂'! multidia_duality!) this;
-          have : H ⊢! ∼⋀Δ ➝ □^[n](∼⋀◇'⁻¹^[n]Δ) := contra₂'! this;
-          have : H ⊢! (⋀Δ ➝ ⊥) ➝ □^[n](∼⋀◇'⁻¹^[n]Δ) := imp_trans''! (and₂'! neg_equiv!) this;
-          have : H ⊢! ⋀Γ ➝ □^[n](∼⋀◇'⁻¹^[n]Δ) := imp_trans''! d₁ this;
-          have : H ⊢! □⋀Γ ➝ □^[(n + 1)](∼⋀◇'⁻¹^[n]Δ) := by simpa using imply_box_distribute'! this;
+          have : 𝓢 ⊢! ◇^[n]⋀◇'⁻¹^[n]Δ ➝ ⋀Δ := imp_trans''! iff_conjmultidia_multidiaconj! $ this;
+          have : 𝓢 ⊢! ∼(□^[n](∼⋀◇'⁻¹^[n]Δ)) ➝ ⋀Δ := imp_trans''! (and₂'! multidia_duality!) this;
+          have : 𝓢 ⊢! ∼⋀Δ ➝ □^[n](∼⋀◇'⁻¹^[n]Δ) := contra₂'! this;
+          have : 𝓢 ⊢! (⋀Δ ➝ ⊥) ➝ □^[n](∼⋀◇'⁻¹^[n]Δ) := imp_trans''! (and₂'! neg_equiv!) this;
+          have : 𝓢 ⊢! ⋀Γ ➝ □^[n](∼⋀◇'⁻¹^[n]Δ) := imp_trans''! d₁ this;
+          have : 𝓢 ⊢! □⋀Γ ➝ □^[(n + 1)](∼⋀◇'⁻¹^[n]Δ) := by simpa using imply_box_distribute'! this;
           exact iff_mem_neg.mp $ h $ membership_iff.mpr $ (Context.of! this) ⨀ dΓconj;
         }
 
@@ -80,32 +80,36 @@ lemma multirel_def_multibox : Ω₁ ≺^[n] Ω₂ ↔ ∀ {φ}, □^[n]φ ∈ Ω
         apply hΩ;
         simp_all;
 
-lemma multirel_def_multibox' : Ω₁ ≺^[n] Ω₂ ↔ ∀ {φ}, φ ∈ (□''⁻¹^[n]Ω₁.theory) → φ ∈ Ω₂.theory := by
+lemma multirel_def_multibox' : Ω₁ ≺^[n] Ω₂ ↔ ∀ {φ}, φ ∈ (□''⁻¹^[n]Ω₁.1) → φ ∈ Ω₂.1 := by
   constructor;
   . intro h φ hp; exact multirel_def_multibox.mp h hp;
   . intro h; apply multirel_def_multibox.mpr; assumption;
 
-lemma multirel_def_multidia : Ω₁ ≺^[n] Ω₂ ↔ ∀ {φ}, (φ ∈ Ω₂.theory → ◇^[n]φ ∈ Ω₁.theory) := Iff.trans multirel_def_multibox multibox_multidia
+lemma multirel_def_multidia : Ω₁ ≺^[n] Ω₂ ↔ ∀ {φ}, (φ ∈ Ω₂.1 → ◇^[n]φ ∈ Ω₁.1) := Iff.trans multirel_def_multibox multibox_multidia
 
-lemma rel_def_dia : Ω₁ ≺ Ω₂ ↔ ∀ {φ}, φ ∈ Ω₂.theory → ◇φ ∈ Ω₁.theory := by simpa using multirel_def_multidia (n := 1) (Ω₁ := Ω₁) (Ω₂ := Ω₂)
+lemma rel_def_dia : Ω₁ ≺ Ω₂ ↔ ∀ {φ}, φ ∈ Ω₂.1 → ◇φ ∈ Ω₁.1 := by simpa using multirel_def_multidia (n := 1) (Ω₁ := Ω₁) (Ω₂ := Ω₂)
 
 end canonicalFrame
 
 
-abbrev canonicalModel (H : Hilbert ℕ) [H.IsNormal] [H.Consistent] : Model where
-  toFrame := canonicalFrame H
-  Val Ω a := (atom a) ∈ Ω.theory
+abbrev canonicalModel (𝓢 : S) [System.Consistent 𝓢] [System.K 𝓢] : Model where
+  toFrame := canonicalFrame 𝓢
+  Val Ω a := (atom a) ∈ Ω.1
 
 @[reducible]
-instance : Semantics (Formula ℕ) (canonicalModel H).World := Formula.Kripke.Satisfies.semantics (M := canonicalModel H)
+instance : Semantics (Formula ℕ) (canonicalModel 𝓢).World := Formula.Kripke.Satisfies.semantics (M := canonicalModel 𝓢)
 
 
 section lemmata
 
 variable {φ ψ : Formula ℕ}
 
-lemma truthlemma : ∀ {Ω : (canonicalModel H).World}, Ω ⊧ φ ↔ (φ ∈ Ω.theory) := by
+lemma truthlemma : ∀ {Ω : (canonicalModel 𝓢).World}, Ω ⊧ φ ↔ (φ ∈ Ω.1) := by
   induction φ using Formula.rec' with
+  | hatom => simp_all [Semantics.Realize, Kripke.Satisfies];
+  | hfalsum =>
+    simp only [Semantics.Realize, Satisfies, false_iff];
+    exact not_mem_falsum;
   | hbox φ ih =>
     intro Ω;
     constructor;
@@ -128,65 +132,45 @@ lemma truthlemma : ∀ {Ω : (canonicalModel H).World}, Ω ⊧ φ ↔ (φ ∈ Ω
       have := iff_mem_imp.mp h;
       intro hp; replace hp := ihp.mp hp;
       exact ihq.mpr $ this hp
-  | _ => simp_all [Semantics.Realize, Kripke.Satisfies];
 
 
-lemma iff_valid_on_canonicalModel_deducible : (canonicalModel H) ⊧ φ ↔ H ⊢! φ := by
+lemma iff_valid_on_canonicalModel_deducible : (canonicalModel 𝓢) ⊧ φ ↔ 𝓢 ⊢! φ := by
   constructor;
   . contrapose;
     intro h;
-    have : Theory.Consistent H ({∼φ}) := by
-      apply Theory.def_consistent.mpr;
+    have : FormulaSet.Consistent 𝓢 ({∼φ}) := by
+      apply FormulaSet.def_consistent.mpr;
       intro Γ hΓ;
       by_contra hC;
-      have : H ⊢! φ := dne'! $ neg_equiv'!.mpr $ replace_imply_left_conj! hΓ hC;
+      have : 𝓢 ⊢! φ := dne'! $ neg_equiv'!.mpr $ replace_imply_left_conj! hΓ hC;
       contradiction;
     obtain ⟨Ω, hΩ⟩ := lindenbaum this;
-    apply not_validOnModel_of_exists_world;
+    apply ValidOnModel.not_of_exists_world;
     use Ω;
     exact truthlemma.not.mpr $ iff_mem_neg.mp (by tauto_set);
   . intro h Ω;
-    suffices φ ∈ Ω.theory by exact truthlemma.mpr this;
+    suffices φ ∈ Ω.1 by exact truthlemma.mpr this;
     by_contra hC;
-    obtain ⟨Γ, hΓ₁, hΓ₂⟩ := Theory.iff_insert_inconsistent.mp $ (MaximalConsistentTheory.maximal' hC);
-    have : Γ ⊢[H]! ⊥ := FiniteContext.provable_iff.mpr $ and_imply_iff_imply_imply'!.mp hΓ₂ ⨀ h;
-    have : Γ ⊬[H] ⊥ := Theory.def_consistent.mp Ω.consistent _ hΓ₁;
+    obtain ⟨Γ, hΓ₁, hΓ₂⟩ := FormulaSet.iff_insert_inconsistent.mp $ (Ω.maximal' hC);
+    have : Γ ⊢[𝓢]! ⊥ := FiniteContext.provable_iff.mpr $ and_imply_iff_imply_imply'!.mp hΓ₂ ⨀ h;
+    have : Γ ⊬[𝓢] ⊥ := FormulaSet.def_consistent.mp (Ω.consistent) _ hΓ₁;
     contradiction;
-
-lemma realize_axiomset_of_self_canonicalModel : (canonicalModel H) ⊧* H.axioms := by
-  apply Semantics.realizeSet_iff.mpr;
-  intro φ hp;
-  apply iff_valid_on_canonicalModel_deducible.mpr;
-  exact maxm! hp;
-
-lemma realize_theory_of_self_canonicalModel : (canonicalModel H) ⊧* (System.theory H) := by
-  apply Semantics.realizeSet_iff.mpr;
-  intro φ hp;
-  apply iff_valid_on_canonicalModel_deducible.mpr;
-  simpa [System.theory] using hp;
-
-lemma complete_of_canonical {C : FrameClass} (hFC : canonicalFrame H ∈ C) : C ⊧ φ → H ⊢! φ := by
-  contrapose;
-  intro h;
-  apply not_validOnFrameClass_of_exists_model;
-  use (canonicalModel H);
-  constructor;
-  . assumption;
-  . exact iff_valid_on_canonicalModel_deducible.not.mpr h;
-
-lemma instCompleteOfCanonical {C : FrameClass} (hC : (Kripke.canonicalFrame H) ∈ C) : Complete H C := ⟨complete_of_canonical hC⟩
 
 end lemmata
 
+class Canonical (𝓢 : S) [System.Consistent 𝓢] [System.K 𝓢] (C : FrameClass) : Prop where
+  canonical : (Kripke.canonicalFrame 𝓢) ∈ C
+
+instance [Canonical 𝓢 C] : Complete 𝓢 C := ⟨by
+  contrapose;
+  intro h;
+  apply ValidOnFrameClass.not_of_exists_model;
+  use (canonicalModel 𝓢);
+  constructor;
+  . exact Canonical.canonical;
+  . exact iff_valid_on_canonicalModel_deducible.not.mpr h;
+⟩
+
 end Kripke
-
-
-namespace K
-
-instance Kripke.complete : Complete (Hilbert.K ℕ) (Kripke.AllFrameClass) := Hilbert.Kripke.instCompleteOfCanonical (C := Kripke.AllFrameClass) $ by tauto
-
-end K
-
-end Hilbert
 
 end LO.Modal
