Foundation/Modal/Kripke/Preservation.lean
@@ -1,12 +1,10 @@
 import Foundation.Modal.Kripke.Closure
 
-
 namespace LO.Modal
 
 namespace Kripke
 
 open Formula.Kripke
-
 
 section Bisimulation
 
@@ -122,14 +120,13 @@ def id : M →ₚ M where
   back := by simp;
   atomic := by simp;
 
-def mkAtomic (f : M₁.toFrame →ₚ M₂.toFrame) (atomic : ∀ {w a}, (M₁ w a) ↔ (M₂ (f w) a)) : M₁ →ₚ M₂ := {
-  toFun := f,
-  forth := f.forth,
-  back := f.back,
-  atomic := atomic,
-}
+def ofAtomic (f : M₁.toFrame →ₚ M₂.toFrame) (atomic : ∀ {w a}, (M₁ w a) ↔ (M₂ (f w) a)) : M₁ →ₚ M₂ where
+  toFun := f
+  forth := f.forth
+  back := f.back
+  atomic := atomic
 
-def comp (f : M₁ →ₚ M₂) (g : M₂ →ₚ M₃) : M₁ →ₚ M₃ := mkAtomic (f.toPseudoEpimorphism.comp (g.toPseudoEpimorphism)) $ by
+def comp (f : M₁ →ₚ M₂) (g : M₂ →ₚ M₃) : M₁ →ₚ M₃ := ofAtomic (f.toPseudoEpimorphism.comp (g.toPseudoEpimorphism)) $ by
   intro x φ;
   constructor;
   . intro h;
@@ -141,8 +138,8 @@ def comp (f : M₁ →ₚ M₂) (g : M₂ →ₚ M₃) : M₁ →ₚ M₃ := mkA
     apply g.atomic.mpr;
     assumption;
 
-def bisimulation (f : M₁ →ₚ M₂) : M₁ ⇄ M₂ := {
-  toRel := Function.graph f,
+def bisimulation (f : M₁ →ₚ M₂) : M₁ ⇄ M₂ where
+  toRel := Function.graph f
   atomic := by
     rintro x₁ x₂ a rfl;
     constructor;
@@ -157,7 +154,6 @@ def bisimulation (f : M₁ →ₚ M₂) : M₁ ⇄ M₂ := {
     rintro x₁ x₂ y₂ rfl rx₂y₂;
     obtain ⟨y₁, ⟨rfl, _⟩⟩ := f.back rx₂y₂;
     use y₁;
-}
 
 lemma modal_equivalence (f : M₁ →ₚ M₂) (w : M₁.World) : w ↭ (f w) := by
   apply modal_equivalent_of_bisimilar $ Model.PseudoEpimorphism.bisimulation f;
@@ -171,10 +167,10 @@ variable {F₁ F₂ : Kripke.Frame} {M₁ M₂ : Kripke.Model}
 lemma validOnFrame_of_surjective_pseudoMorphism (f : F₁ →ₚ F₂) (f_surjective : Function.Surjective f) : F₁ ⊧ φ → F₂ ⊧ φ := by
   contrapose;
   intro h;
-  obtain ⟨V₂, w₂, h⟩ := exists_valuation_world_of_not_validOnFrame_of h;
+  obtain ⟨V₂, w₂, h⟩ := ValidOnFrame.exists_valuation_world_of_not h;
   obtain ⟨w₁, rfl⟩ := f_surjective w₂;
 
-  apply not_validOnFrame_of_exists_valuation_world;
+  apply ValidOnFrame.not_of_exists_valuation_world;
   let V₁ := λ w a => V₂ (f w) a;
   use V₁, w₁;
 
