Foundation.lean
@@ -65,60 +65,34 @@ import Foundation.IntProp.Dialectica.Basic
 
 -- Modal
 
-import Foundation.Modal.Hilbert.GL_Independency
-import Foundation.Modal.Hilbert.Subst
-import Foundation.Modal.Hilbert.Maximal.Unprovability
+import Foundation.Modal.Hilbert.KP
+import Foundation.Modal.Hilbert.S5Grz
+import Foundation.Modal.Hilbert.GL.Alternatives
+import Foundation.Modal.Hilbert.GL.Independency
 
-import Foundation.Modal.Hilbert.WeakerThan.GL_GLS
-import Foundation.Modal.Hilbert.WeakerThan.K_K4
-import Foundation.Modal.Hilbert.WeakerThan.K_K5
-import Foundation.Modal.Hilbert.WeakerThan.K_KB
-import Foundation.Modal.Hilbert.WeakerThan.K_KD
-import Foundation.Modal.Hilbert.WeakerThan.K4_GL
-import Foundation.Modal.Hilbert.WeakerThan.K4_Grz
-import Foundation.Modal.Hilbert.WeakerThan.K4_K45
-import Foundation.Modal.Hilbert.WeakerThan.K4_KD4
-import Foundation.Modal.Hilbert.WeakerThan.K4_S4
-import Foundation.Modal.Hilbert.WeakerThan.K4_Triv
-import Foundation.Modal.Hilbert.WeakerThan.K45_KB4
-import Foundation.Modal.Hilbert.WeakerThan.K5_K45
-import Foundation.Modal.Hilbert.WeakerThan.K5_KD5
-import Foundation.Modal.Hilbert.WeakerThan.KB_KDB
-import Foundation.Modal.Hilbert.WeakerThan.KB5_S5
-import Foundation.Modal.Hilbert.WeakerThan.KD_KDB
-import Foundation.Modal.Hilbert.WeakerThan.KD_KT
-import Foundation.Modal.Hilbert.WeakerThan.KD4_KD45
-import Foundation.Modal.Hilbert.WeakerThan.KD45_S5
-import Foundation.Modal.Hilbert.WeakerThan.KD5_KD45
-import Foundation.Modal.Hilbert.WeakerThan.KDB_KTB
-import Foundation.Modal.Hilbert.WeakerThan.KT_Grz
-import Foundation.Modal.Hilbert.WeakerThan.KT_KTB
-import Foundation.Modal.Hilbert.WeakerThan.KT_S4
-import Foundation.Modal.Hilbert.WeakerThan.KTB_S5
-import Foundation.Modal.Hilbert.WeakerThan.S4_S5
+import Foundation.Modal.Kripke.Hilbert.K
+import Foundation.Modal.Kripke.Hilbert.KT
+import Foundation.Modal.Kripke.Hilbert.KTB
+import Foundation.Modal.Kripke.Hilbert.KT4B
+import Foundation.Modal.Kripke.Hilbert.S4
+import Foundation.Modal.Kripke.Hilbert.S4Dot2
+import Foundation.Modal.Kripke.Hilbert.S4Dot3
+import Foundation.Modal.Kripke.Hilbert.S5
+import Foundation.Modal.Kripke.Hilbert.Triv
+import Foundation.Modal.Kripke.Hilbert.Ver
 
-import Foundation.Modal.Hilbert.Equiv.GL
-import Foundation.Modal.Hilbert.Equiv.KD_KP
-import Foundation.Modal.Hilbert.Equiv.S5_KT4B
-import Foundation.Modal.Hilbert.Equiv.S5Grz_Triv
+import Foundation.Modal.Kripke.Hilbert.GL.Unnecessitation
+import Foundation.Modal.Kripke.Hilbert.GL.MDP
+
+import Foundation.Modal.Kripke.Hilbert.Grz.Completeness
+
+import Foundation.Modal.Kripke.NNFormula
+import Foundation.Modal.Kripke.ComplexityLimited
+import Foundation.Modal.Kripke.Undefinability
+
+import Foundation.Modal.PLoN.Hilbert.N
 
 import Foundation.Modal.ModalCompanion.GMT
 
 import Foundation.Modal.Boxdot.K4_S4
 import Foundation.Modal.Boxdot.GL_Grz
-
-import Foundation.Modal.Kripke.NNFormula
-import Foundation.Modal.Kripke.Filteration
-import Foundation.Modal.Kripke.ComplexityLimited
-import Foundation.Modal.Kripke.Ver
-import Foundation.Modal.Kripke.Dot3
-import Foundation.Modal.Kripke.S5
-import Foundation.Modal.Kripke.Undefinability
-
-import Foundation.Modal.Kripke.GL.Tree
-import Foundation.Modal.Kripke.GL.Unnec
-import Foundation.Modal.Kripke.GL.MDP
-
-import Foundation.Modal.Kripke.Grz.Completeness
-
-import Foundation.Modal.PLoN.Completeness
