Foundation/Modal/Boxdot/Basic.lean
@@ -16,20 +16,19 @@ def Formula.BoxdotTranslation : Formula α → Formula α
   | □φ => ⊡(BoxdotTranslation φ)
 postfix:90 "ᵇ" => Formula.BoxdotTranslation
 
-
 class BoxdotProperty (H₁ H₂ : Hilbert α) where
   bdp {φ} : H₁ ⊢! φᵇ ↔ H₂ ⊢! φ
 
-theorem boxdotTranslated
-  {H₁ H₂ : Hilbert α} [H₁.IsNormal] [H₂.IsNormal]
-  (h : ∀ φ ∈ H₁.axioms, H₂ ⊢! φᵇ) : H₁ ⊢! φ → H₂ ⊢! φᵇ := by
+theorem boxdotTranslated {H₁ H₂ : Hilbert α}
+  [System.K H₂]
+  (h : ∀ φ ∈ H₁.axiomInstances, H₂ ⊢! φᵇ) : H₁ ⊢! φ → H₂ ⊢! φᵇ := by
   intro d;
-  induction d using inducition_with_necOnly! with
-  | hMaxm hs => exact h _ hs;
-  | hNec ihp => exact boxdot_nec! $ ihp;
-  | hMdp ihpq ihp => exact ihpq ⨀ ihp;
-  | hElimContra => exact elim_contra!;
-  | hImply₂ => exact imply₂!;
-  | hImply₁ => exact imply₁!;
+  induction d using Hilbert.Deduction.rec! with
+  | maxm hs => exact h _ hs;
+  | mdp ihpq ihp => exact ihpq ⨀ ihp;
+  | nec ihp => exact boxdot_nec! $ ihp;
+  | imply₂ => exact imply₂!;
+  | imply₁ => exact imply₁!;
+  | ec => exact elim_contra!;
 
 end LO.Modal
