Foundation/Modal/Kripke/Filteration.lean
@@ -1,6 +1,6 @@
 import Mathlib.Data.Set.Finite.Powerset
-import Foundation.Modal.Kripke.Geach.Systems
 import Foundation.Modal.Kripke.Closure
+import Foundation.Modal.Subformulas
 
 universe u v
 
@@ -10,23 +10,14 @@ namespace Kripke
 
 open Formula (atom)
 open Formula.Kripke
-
-section
-
-abbrev ReflexiveSymmetricFiniteFrameClass : FiniteFrameClass := { F | Reflexive F.Rel ∧ Symmetric F.Rel }
-
-abbrev ReflexiveTransitiveFiniteFrameClass : FiniteFrameClass := { F | Reflexive F.Rel ∧ Transitive F.Rel }
-
-abbrev ReflexiveTransitiveSymmetricFiniteFrameClass : FiniteFrameClass := { F | Reflexive F.Rel ∧ Transitive F.Rel ∧ Symmetric F.Rel }
-
-end
+open FormulaSet.SubformulaClosed
 
 
 section
 
-def filterEquiv (M : Kripke.Model) (T : Theory ℕ) [T.SubformulaClosed] (x y : M.World) := ∀ φ, (_ : φ ∈ T := by trivial) → x ⊧ φ ↔ y ⊧ φ
+def filterEquiv (M : Kripke.Model) (T : FormulaSet ℕ) [T.SubformulaClosed] (x y : M.World) := ∀ φ, (_ : φ ∈ T := by trivial) → x ⊧ φ ↔ y ⊧ φ
 
-variable (M : Kripke.Model) (T : Theory ℕ) [T.SubformulaClosed]
+variable (M : Kripke.Model) (T : FormulaSet ℕ) [T.SubformulaClosed]
 
 lemma filterEquiv.equivalence : Equivalence (filterEquiv M T) where
   refl := by intro x φ _; rfl;
@@ -69,15 +60,15 @@ lemma FilterEqvQuotient.finite (T_finite : T.Finite) : Finite (FilterEqvQuotient
 
 instance : Nonempty (FilterEqvQuotient M T) := ⟨⟦M.toFrame.world_nonempty.some⟧⟩
 
-class FilterOf (FM : Model) (M : Model) (T : Theory ℕ) [T.SubformulaClosed] : Prop where
+class FilterOf (FM : Model) (M : Model) (T : FormulaSet ℕ) [T.SubformulaClosed] : Prop where
   def_world : FM.World = FilterEqvQuotient M T := by rfl
   def_rel₁ : ∀ {x y : M.toFrame}, x ≺ y → Frame.Rel' (cast def_world.symm ⟦x⟧) (cast def_world.symm ⟦y⟧) := by tauto;
   def_box : ∀ {Qx Qy : FM.World}, Qx ≺ Qy → Quotient.lift₂ (λ x y => ∀ φ, □φ ∈ T → (x ⊧ □φ → y ⊧ φ)) (by
     intro x₁ y₁ x₂ y₂ hx hy;
     apply eq_iff_iff.mpr;
     constructor;
-    . intro h φ hp sp₂; exact hy φ |>.mp $ h φ hp $ hx (□φ) hp |>.mpr sp₂;
-    . intro h φ hp sp₁; exact hy φ |>.mpr $ h φ hp $ hx (□φ) hp |>.mp sp₁;
+    . intro h φ hp sp₂; exact hy φ (FormulaSet.SubformulaClosed.mem_box hp) |>.mp $ h φ hp $ hx (□φ) hp |>.mpr sp₂;
+    . intro h φ hp sp₁; exact hy φ (FormulaSet.SubformulaClosed.mem_box hp) |>.mpr $ h φ hp $ hx (□φ) hp |>.mp sp₁;
   ) (cast def_world Qx) (cast def_world Qy)
   def_valuation Qx a : (ha : (atom a) ∈ T := by trivial) →
     FM Qx a ↔ Quotient.lift (λ x => M x a) (by
@@ -119,30 +110,30 @@ abbrev standardFilterationValuation (Qx : FilterEqvQuotient M T) (a : ℕ) := (h
 ) Qx
 
 
-abbrev coarsestFilterationFrame (M : Model) (T : Theory ℕ) [T.SubformulaClosed] : Kripke.Frame where
+abbrev coarsestFilterationFrame (M : Model) (T : FormulaSet ℕ) [T.SubformulaClosed] : Kripke.Frame where
   World := FilterEqvQuotient M T
   Rel Qx Qy :=
     Quotient.lift₂ (λ x y => ∀ φ, □φ ∈ T → (x ⊧ □φ → y ⊧ φ)) (by
       intro x₁ y₁ x₂ y₂ hx hy;
       apply eq_iff_iff.mpr;
       constructor;
-      . intro h φ hp sp₂; exact hy φ |>.mp $ h φ hp $ hx (□φ) hp |>.mpr sp₂;
-      . intro h φ hp sp₁; exact hy φ |>.mpr $ h φ hp $ hx (□φ) hp |>.mp sp₁;
+      . intro h φ hp sp₂; exact hy φ (FormulaSet.SubformulaClosed.mem_box hp) |>.mp $ h φ hp $ hx (□φ) hp |>.mpr sp₂;
+      . intro h φ hp sp₁; exact hy φ (FormulaSet.SubformulaClosed.mem_box hp) |>.mpr $ h φ hp $ hx (□φ) hp |>.mp sp₁;
     ) Qx Qy
 
-abbrev coarsestFilterationModel (M : Model) (T : Theory ℕ) [T.SubformulaClosed] : Kripke.Model where
+abbrev coarsestFilterationModel (M : Model) (T : FormulaSet ℕ) [T.SubformulaClosed] : Kripke.Model where
   toFrame := coarsestFilterationFrame M T
   Val := standardFilterationValuation M T
 
-instance coarsestFilterationModel.filterOf {M} {T : Theory ℕ} [T.SubformulaClosed] : FilterOf (coarsestFilterationModel M T) M T where
+instance coarsestFilterationModel.filterOf {M} {T : FormulaSet ℕ} [T.SubformulaClosed] : FilterOf (coarsestFilterationModel M T) M T where
   def_box := by tauto
 
 
-abbrev finestFilterationFrame (M : Model) (T : Theory ℕ) [T.SubformulaClosed] : Kripke.Frame where
+abbrev finestFilterationFrame (M : Model) (T : FormulaSet ℕ) [T.SubformulaClosed] : Kripke.Frame where
   World := FilterEqvQuotient M T
   Rel Qx Qy := ∃ x y, Qx = ⟦x⟧ ∧ Qy = ⟦y⟧ ∧ x ≺ y
 
-abbrev finestFilterationModel (M : Model) (T : Theory ℕ) [T.SubformulaClosed] : Kripke.Model where
+abbrev finestFilterationModel (M : Model) (T : FormulaSet ℕ) [T.SubformulaClosed] : Kripke.Model where
   toFrame := finestFilterationFrame M T
   Val := standardFilterationValuation M T
 
@@ -165,7 +156,7 @@ lemma symmetric_of_symmetric (hSymm : Symmetric M.toFrame) : Symmetric (finestFi
 end finestFilterationModel
 
 
-abbrev finestFilterationTransitiveClosureModel (M : Model) (T : Theory ℕ) [T.SubformulaClosed] : Kripke.Model where
+abbrev finestFilterationTransitiveClosureModel (M : Model) (T : FormulaSet ℕ) [T.SubformulaClosed] : Kripke.Model where
   toFrame := (finestFilterationFrame M T)^+
   Val := standardFilterationValuation M T
 
@@ -214,7 +205,7 @@ end
 
 section
 
-variable {M : Model} {T : Theory ℕ} [T.SubformulaClosed]
+variable {M : Model} {T : FormulaSet ℕ} [T.SubformulaClosed]
          (FM : Model) (filterOf : FilterOf FM M T)
 
 theorem filteration {x : M.World} {φ : Formula ℕ} (hs : φ ∈ T) : x ⊧ φ ↔ (cast (filterOf.def_world.symm) ⟦x⟧) ⊧ φ := by
@@ -227,129 +218,20 @@ theorem filteration {x : M.World} {φ : Formula ℕ} (hs : φ ∈ T) : x ⊧ φ 
     . intro h Qy rQxQy;
       obtain ⟨y, ey⟩ := Quotient.exists_rep (cast (filterOf.def_world) Qy);
       have this := filterOf.def_box rQxQy; simp [←ey] at this;
-      simpa [ey] using ihp (Theory.SubformulaClosed.mem_box hs) |>.mp $ @this φ hs h;
+      simpa [ey] using ihp (FormulaSet.SubformulaClosed.mem_box hs) |>.mp $ @this φ hs h;
     . intro h y rxy;
       have rQxQy := filterOf.def_rel₁ rxy;
-      exact ihp (Theory.SubformulaClosed.mem_box hs) |>.mpr $ h _ rQxQy;
+      exact ihp (FormulaSet.SubformulaClosed.mem_box hs) |>.mpr $ h _ rQxQy;
   | himp φ ψ ihp ihq =>
     constructor;
     . rintro hxy hp;
-      exact (ihq (by trivial) |>.mp $ hxy (ihp (Theory.SubformulaClosed.mem_imp₁ hs) |>.mpr hp));
+      exact ihq (FormulaSet.SubformulaClosed.mem_imp₂ hs) |>.mp $ hxy (ihp (FormulaSet.SubformulaClosed.mem_imp₁ hs) |>.mpr hp);
     . rintro hxy hp;
-      exact (ihq (by trivial) |>.mpr $ hxy (ihp (Theory.SubformulaClosed.mem_imp₁ hs) |>.mp hp));
+      exact ihq (FormulaSet.SubformulaClosed.mem_imp₂ hs) |>.mpr $ hxy (ihp (FormulaSet.SubformulaClosed.mem_imp₁ hs) |>.mp hp);
   | _ => trivial
 
 end
 
 end Kripke
-
-
-namespace Hilbert
-
-open Modal.Kripke
-open Hilbert.Kripke
-
-instance K.Kripke.finite_complete : Complete (Hilbert.K ℕ) (AllFiniteFrameClass) := ⟨by
-  intro φ hp;
-  apply Hilbert.K.Kripke.complete.complete;
-  intro F _ V x;
-  let M : Kripke.Model := ⟨F, V⟩;
-  let FM := coarsestFilterationModel M ↑φ.subformulae;
-
-  apply filteration FM (coarsestFilterationModel.filterOf) (by aesop) |>.mpr;
-  apply hp (by
-    suffices Finite (FilterEqvQuotient M φ.subformulae) by
-      simp only [FiniteFrameClass.toFrameClass, AllFiniteFrameClass, Set.image_univ, Set.mem_range];
-      use ⟨FM.toFrame⟩;
-    apply FilterEqvQuotient.finite;
-    simp;
-  ) FM.Val
-⟩
-
-instance K.Kripke.ffp : FiniteFrameProperty (Hilbert.K ℕ) AllFiniteFrameClass where
-  complete := K.Kripke.finite_complete
-  sound := Kripke.instFiniteSound_of_instSound (C := AllFrameClass) (FC := AllFiniteFrameClass) rfl
-
-
-instance KTB.Kripke.finite_complete : Complete (Hilbert.KTB ℕ) (ReflexiveSymmetricFiniteFrameClass) := ⟨by
-  intro φ hp;
-  apply Hilbert.KTB.Kripke.complete.complete;
-  intro F ⟨F_refl, F_symm⟩ V x;
-  let M : Kripke.Model := ⟨F, V⟩;
-  let FM := finestFilterationModel M φ.subformulae;
-  apply filteration FM (finestFilterationModel.filterOf) (by aesop) |>.mpr;
-  apply hp (by
-    suffices Finite (FilterEqvQuotient M φ.subformulae) by
-      simp only [FiniteFrameClass.toFrameClass, ReflexiveSymmetricFiniteFrameClass, Set.mem_image, Set.mem_setOf_eq];
-      use ⟨FM.toFrame⟩;
-      refine ⟨⟨?_, ?_⟩, ?_⟩;
-      . apply reflexive_filterOf_of_reflexive (finestFilterationModel.filterOf);
-        exact F_refl;
-      . apply finestFilterationModel.symmetric_of_symmetric;
-        exact F_symm;
-      . rfl;
-    apply FilterEqvQuotient.finite;
-    simp;
-  ) FM.Val
-⟩
-
-instance KTB.Kripke.ffp : FiniteFrameProperty (Hilbert.KTB ℕ) ReflexiveSymmetricFiniteFrameClass where
-  complete := KTB.Kripke.finite_complete
-  sound := Kripke.instFiniteSound_of_instSound (C := ReflexiveSymmetricFrameClass) (FC := ReflexiveSymmetricFiniteFrameClass) rfl
-
-
-open finestFilterationTransitiveClosureModel in
-instance S4.Kripke.finite_complete : Complete (Hilbert.S4 ℕ) (ReflexiveTransitiveFiniteFrameClass) := ⟨by
-  intro φ hp;
-  apply Hilbert.S4.Kripke.complete.complete;
-  intro F ⟨F_refl, F_trans⟩ V x;
-  let M : Kripke.Model := ⟨F, V⟩;
-  let FM := finestFilterationTransitiveClosureModel M φ.subformulae;
-  apply @filteration M φ.subformulae _ FM ?filterOf x φ (by simp) |>.mpr;
-  apply hp (by
-    suffices Finite (FilterEqvQuotient M φ.subformulae) by
-      simp only [FiniteFrameClass.toFrameClass];
-      use ⟨FM.toFrame⟩;
-      refine ⟨⟨?_, transitive⟩, rfl⟩;
-      . exact reflexive_of_transitive_reflexive (by apply F_trans) F_refl;
-    apply FilterEqvQuotient.finite;
-    simp;
-  ) FM.Val;
-  . apply finestFilterationTransitiveClosureModel.filterOf;
-    exact F_trans;
-⟩
-
-instance S4.Kripke.ffp : FiniteFrameProperty (Hilbert.S4 ℕ) ReflexiveTransitiveFiniteFrameClass where
-  complete := S4.Kripke.finite_complete
-  sound := Kripke.instFiniteSound_of_instSound (C := ReflexiveTransitiveFrameClass) (FC := ReflexiveTransitiveFiniteFrameClass) rfl
-
-
-open finestFilterationTransitiveClosureModel in
-instance KT4B.Kripke.finite_complete : Complete (Hilbert.KT4B ℕ) (ReflexiveTransitiveSymmetricFiniteFrameClass) := ⟨by
-  intro φ hp;
-  apply Hilbert.KT4B.Kripke.complete.complete;
-  intro F ⟨F_refl, F_trans, F_symm⟩ V x;
-  let M : Kripke.Model := ⟨F, V⟩;
-  let FM := finestFilterationTransitiveClosureModel M φ.subformulae;
-  apply @filteration M φ.subformulae _ FM ?filterOf x φ (by simp) |>.mpr;
-  apply hp (by
-    suffices Finite (FilterEqvQuotient M φ.subformulae) by
-      simp only [FiniteFrameClass.toFrameClass, Set.mem_image, Set.mem_setOf_eq];
-      use ⟨FM.toFrame⟩;
-      refine ⟨⟨?refl, transitive, ?symm⟩, rfl⟩;
-      . exact reflexive_of_transitive_reflexive (by apply F_trans) F_refl;
-      . exact symmetric_of_symmetric F_symm;
-    apply FilterEqvQuotient.finite;
-    simp;
-  ) FM.Val;
-  . apply finestFilterationTransitiveClosureModel.filterOf
-    exact F_trans;
-⟩
-
-instance KT4B.Kripke.ffp : FiniteFrameProperty (Hilbert.KT4B ℕ) ReflexiveTransitiveSymmetricFiniteFrameClass where
-  complete := KT4B.Kripke.finite_complete
-  sound := Kripke.instFiniteSound_of_instSound (C := ReflexiveTransitiveSymmetricFrameClass) (FC := ReflexiveTransitiveSymmetricFiniteFrameClass) rfl
-
-end Hilbert
 
 end LO.Modal
