Foundation/Modal/PLoN/Basic.lean
@@ -1,0 +1,237 @@
+import Foundation.Modal.Formula
+
+universe u v
+
+namespace LO.Modal
+
+namespace PLoN
+
+structure Frame where
+  World : Type
+  Rel : Formula ℕ → World → World → Prop
+  [World_nonempty : Nonempty World]
+
+noncomputable abbrev Frame.default {F : PLoN.Frame} : F.World := F.World_nonempty.some
+scoped notation "﹫" => Frame.default
+
+
+instance : CoeFun (PLoN.Frame) (λ F => Formula ℕ → F.World → F.World → Prop) := ⟨Frame.Rel⟩
+
+abbrev Frame.Rel' {F : PLoN.Frame} (φ : Formula ℕ) (x y : F.World) := F.Rel φ x y
+scoped notation:45 x:90 " ≺[" φ "] " y:90 => Frame.Rel' φ x y
+
+
+structure FiniteFrame extends Frame where
+  [World_finite : Finite World]
+
+instance : Coe (FiniteFrame) (Frame) := ⟨λ F ↦ F.toFrame⟩
+
+
+abbrev terminalFrame : FiniteFrame where
+  World := Unit
+  Rel := λ _ _ _ => True
+
+
+abbrev FrameClass := Set (PLoN.Frame)
+
+
+abbrev Valuation (F : PLoN.Frame) := F.World → ℕ → Prop
+
+structure Model extends PLoN.Frame where
+  Valuation : PLoN.Valuation toFrame
+
+end PLoN
+
+
+
+open PLoN
+
+namespace Formula.PLoN
+
+def Satisfies (M : PLoN.Model) (w : M.World) : Formula ℕ → Prop
+  | atom a  => M.Valuation w a
+  | falsum  => False
+  | φ ➝ ψ => (Satisfies M w φ) → (Satisfies M w ψ)
+  | □φ   => ∀ {w'}, w ≺[φ] w' → (Satisfies M w' φ)
+
+namespace Satisfies
+
+protected instance semantics (M : PLoN.Model) : Semantics (Formula ℕ) (M.World) := ⟨fun w ↦ Formula.PLoN.Satisfies M w⟩
+
+variable {M : PLoN.Model} {x : M.World} {φ ψ : Formula ℕ}
+
+@[simp] protected lemma iff_models : x ⊧ φ ↔ PLoN.Satisfies M x φ := by rfl
+
+lemma box_def : x ⊧ □φ ↔ ∀ y, x ≺[φ] y → y ⊧ φ := by simp [PLoN.Satisfies];
+
+protected lemma not_def : x ⊧ ∼φ ↔ ¬(x ⊧ φ) := by
+  induction φ using Formula.rec' generalizing x with
+  | _ => simp_all [Satisfies];
+
+protected lemma imp_def : x ⊧ φ ➝ ψ ↔ (x ⊧ φ) → (x ⊧ ψ) := by tauto;
+
+protected lemma or_def : x ⊧ φ ⋎ ψ ↔ x ⊧ φ ∨ x ⊧ ψ := by simp [Satisfies]; tauto;
+
+protected lemma and_def : x ⊧ φ ⋏ ψ ↔ x ⊧ φ ∧ x ⊧ ψ := by simp [Satisfies];
+
+protected lemma bot_def : ¬(x ⊧ ⊥) := by simp [Satisfies];
+
+protected lemma top_def : x ⊧ ⊤ := by simp [Satisfies];
+
+instance : Semantics.Tarski M.World where
+  realize_top := λ _ => Satisfies.top_def
+  realize_bot := λ _ => Satisfies.bot_def
+  realize_imp := Satisfies.imp_def
+  realize_not := Satisfies.not_def
+  realize_and := Satisfies.and_def
+  realize_or  := Satisfies.or_def
+
+end Satisfies
+
+
+def ValidOnModel (M : PLoN.Model) (φ : Formula ℕ) : Prop := ∀ w : M.World, w ⊧ φ
+
+namespace ValidOnModel
+
+instance : Semantics (Formula ℕ) (PLoN.Model) := ⟨fun M ↦ Formula.PLoN.ValidOnModel M⟩
+
+@[simp]
+protected lemma iff_models {M : PLoN.Model} {φ : Formula ℕ}
+: M ⊧ φ ↔ Formula.PLoN.ValidOnModel M φ := by rfl
+
+instance : Semantics.Bot (PLoN.Model) where
+  realize_bot _ := by
+    simp [Formula.PLoN.ValidOnModel];
+    use ﹫;
+
+variable {M : PLoN.Model}
+
+protected lemma imply₁ : M ⊧ (Axioms.Imply₁ φ ψ) := by simp [ValidOnModel]; tauto;
+
+protected lemma imply₂ : M ⊧ (Axioms.Imply₂ φ ψ χ) := by simp [ValidOnModel]; tauto;
+
+protected lemma elim_contra : M ⊧ (Axioms.ElimContra φ ψ) := by simp [ValidOnModel]; tauto;
+
+end ValidOnModel
+
+
+def ValidOnFrame (F : PLoN.Frame) (φ : Formula ℕ) := ∀ V, (Model.mk F V) ⊧ φ
+
+namespace ValidOnFrame
+
+instance : Semantics (Formula ℕ) (PLoN.Frame) := ⟨fun F ↦ Formula.PLoN.ValidOnFrame F⟩
+
+@[simp]
+protected lemma iff_models {F : PLoN.Frame} {φ : Formula ℕ}
+: F ⊧ φ ↔ Formula.PLoN.ValidOnFrame F φ := by rfl
+
+variable {F : Frame}
+
+instance : Semantics.Bot (PLoN.Frame) where
+  realize_bot _ := by simp [Formula.PLoN.ValidOnFrame];
+
+protected lemma nec (h : F ⊧ φ) : F ⊧ □φ := by
+  intro V x y _;
+  exact h V y;
+
+protected lemma mdp (hpq : F ⊧ φ ➝ ψ) (hp : F ⊧ φ) : F ⊧ ψ := by
+  intro V x;
+  exact (hpq V x) (hp V x);
+
+protected lemma imply₁ : F ⊧ (Axioms.Imply₁ φ ψ) := by simp [ValidOnFrame]; tauto;
+
+protected lemma imply₂ : F ⊧ (Axioms.Imply₂ φ ψ χ) := by simp [ValidOnFrame]; tauto;
+
+protected lemma elim_contra : F ⊧ (Axioms.ElimContra φ ψ) := by intro V; exact ValidOnModel.elim_contra;
+
+end ValidOnFrame
+
+
+def ValidOnFrameClass (C : PLoN.FrameClass) (φ : Formula ℕ) := ∀ {F}, F ∈ C → F ⊧ φ
+
+namespace ValidOnFrameClass
+
+instance : Semantics (Formula ℕ) (PLoN.FrameClass) := ⟨fun C ↦ Formula.PLoN.ValidOnFrameClass C⟩
+
+variable {C : FrameClass}
+
+@[simp]
+protected lemma iff_models {C : PLoN.FrameClass} {φ : Formula ℕ} : C ⊧ φ ↔ Formula.PLoN.ValidOnFrameClass C φ := by rfl
+
+protected lemma nec (h : C ⊧ φ) : C ⊧ □φ := by
+  intro _ hF;
+  apply PLoN.ValidOnFrame.nec;
+  exact h hF;
+
+protected lemma mdp (hpq : C ⊧ φ ➝ ψ) (hp : C ⊧ φ) : C ⊧ ψ := by
+  intro _ hF;
+  exact PLoN.ValidOnFrame.mdp (hpq hF) (hp hF)
+
+protected lemma imply₁ : C ⊧ (Axioms.Imply₁ φ ψ) := by intro _ _; exact PLoN.ValidOnFrame.imply₁;
+
+protected lemma imply₂ : C ⊧ (Axioms.Imply₂ φ ψ χ) := by intro _ _; exact PLoN.ValidOnFrame.imply₂;
+
+protected lemma elim_contra : C ⊧ (Axioms.ElimContra φ ψ) := by intro _ _; exact PLoN.ValidOnFrame.elim_contra;
+
+
+lemma iff_not_exists_frame : (¬C ⊧ φ) ↔ (∃ F ∈ C, ¬F ⊧ φ) := by
+  apply not_iff_not.mp;
+  push_neg;
+  tauto;
+
+alias ⟨exists_frame_of_not, not_of_exists_frame⟩ := iff_not_exists_frame
+
+
+lemma iff_not_exists_model : (¬C ⊧ φ) ↔ (∃ M : PLoN.Model, M.toFrame ∈ C ∧ ¬M ⊧ φ) := by
+  apply not_iff_not.mp;
+  push_neg;
+  tauto;
+
+alias ⟨exists_model_of_not, not_of_exists_model⟩ := iff_not_exists_model
+
+end ValidOnFrameClass
+
+end Formula.PLoN
+
+
+namespace PLoN.FrameClass
+
+class DefinedBy (C : PLoN.FrameClass) (Γ : Set (Formula ℕ)) where
+  defines : ∀ F, F ∈ C ↔ (∀ φ ∈ Γ, F ⊧ φ)
+
+class IsNonempty (C : PLoN.FrameClass) : Prop where
+  nonempty : Nonempty C
+
+end PLoN.FrameClass
+
+/-
+namespace PLoN
+
+abbrev AllFrameClass (α) : FrameClass α := Set.univ
+
+lemma AllFrameClass.nonempty : (AllFrameClass.{_, 0} α).Nonempty := by
+  use terminalFrame α
+  trivial;
+
+open Formula
+
+lemma N_defines : (Hilbert.N).DefinesPLoNFrameClass (AllFrameClass α) := by
+  intro F;
+  simp [Hilbert.theorems, System.theory, PLoN.ValidOnFrame, PLoN.ValidOnModel];
+  intro φ hp;
+  induction hp using Hilbert.Deduction.inducition_with_necOnly! with
+  | hMaxm h => simp at h;
+  | hMdp ihpq ihp =>
+    intro V w;
+    exact (ihpq V w) (ihp V w)
+  | hNec ihp =>
+    intro V w w' _;
+    exact ihp V w';
+  | _ =>
+    simp_all [PLoN.Satisfies];
+    try tauto;
+
+end PLoN
+-/
+
+end LO.Modal
