Foundation/Modal/Substitution.lean
@@ -1,0 +1,65 @@
+import Foundation.Modal.Formula
+
+namespace LO.Modal
+
+abbrev Substitution (α) := α → (Formula α)
+
+abbrev Substitution.id {α} : Substitution α := λ a => .atom a
+
+namespace Formula
+
+variable {φ ψ : Formula α} {s : Substitution α}
+
+def subst (s : Substitution α) : Formula α → Formula α
+  | atom a  => (s a)
+  | ⊥       => ⊥
+  | □φ      => □(φ.subst s)
+  | φ ➝ ψ   => φ.subst s ➝ ψ.subst s
+
+notation:80 φ "⟦" s "⟧" => Formula.subst s φ
+
+@[simp] lemma subst_atom {a} : (.atom a)⟦s⟧ = s a := rfl
+
+@[simp] lemma subst_bot : ⊥⟦s⟧ = ⊥ := rfl
+
+@[simp] lemma subst_imp : (φ ➝ ψ)⟦s⟧ = φ⟦s⟧ ➝ ψ⟦s⟧ := rfl
+
+@[simp] lemma subst_neg : (∼φ)⟦s⟧ = ∼(φ⟦s⟧) := rfl
+
+@[simp] lemma subst_and : (φ ⋏ ψ)⟦s⟧ = φ⟦s⟧ ⋏ ψ⟦s⟧ := rfl
+
+@[simp] lemma subst_or : (φ ⋎ ψ)⟦s⟧ = φ⟦s⟧ ⋎ ψ⟦s⟧ := rfl
+
+@[simp] lemma subst_iff : (φ ⭤ ψ)⟦s⟧ = (φ⟦s⟧ ⭤ ψ⟦s⟧) := rfl
+
+@[simp] lemma subst_box : (□φ)⟦s⟧ = □(φ⟦s⟧) := rfl
+
+@[simp] lemma subst_multibox : (□^[n]φ)⟦s⟧ = □^[n](φ⟦s⟧) := by
+  induction n with
+  | zero => rfl
+  | succ n ih => simp [ih]
+
+@[simp] lemma subst_dia : (◇φ)⟦s⟧ = ◇(φ⟦s⟧) := rfl
+
+@[simp] lemma subst_multidia : (◇^[n]φ)⟦s⟧ = ◇^[n](φ⟦s⟧) := by
+  induction n with
+  | zero => rfl
+  | succ n ih => simp [ih]
+
+end Formula
+
+
+@[simp] lemma subst_id {φ : Formula α} : φ⟦.id⟧ = φ := by induction φ using Formula.rec' <;> simp_all;
+
+def Substitution.comp (s₁ s₂ : Substitution α) : Substitution α := λ a => (s₁ a)⟦s₂⟧
+infixr:80 " ∘ " => Substitution.comp
+
+@[simp]
+lemma subst_comp {s₁ s₂ : Substitution α} {φ : Formula α} : φ⟦s₁ ∘ s₂⟧ = φ⟦s₁⟧⟦s₂⟧ := by
+  induction φ using Formula.rec' <;> simp_all [Substitution.comp];
+
+class SubstitutionClosed (S : Set (Formula α)) where
+  closed : ∀ φ ∈ S, (∀ s : Substitution α, φ⟦s⟧ ∈ S)
+
+
+end LO.Modal
